FokkerChallenge/EnhancedCslib/List.lean
@@ -13,3 +13,7 @@ theorem foldl_union_replicate_empty {fs : Finset String} (n : ℕ) :
     simp [List.replicate_succ]
     rw [ih]
     grind
+
+lemma union_foldl {l : List _} {fs : Finset String}:
+  fs ⊆ l.foldl Union.union fs := by
+  induction l generalizing fs with grind
